WIP on Clearing admitted properties of IPChecksum.

src/BinEncoders/Env/Examples/IPv4Header.v
@@ -48,13 +48,46 @@ Definition IPv4_Packet :=
           "DestAddress" :: word 32,
           "Options" :: list (word 32)>.
 
-Definition ProtocolTypeCodes : Vector.t (word 16) 3 :=
-  [WO~0~0~0~0~0~0~0~0~0~0~0~0~0~0~0~1;
-   WO~0~0~0~0~0~0~0~0~0~0~0~0~0~1~1~0;
-   WO~0~0~0~0~0~0~0~0~0~0~0~1~0~0~0~1
+Definition ProtocolTypeCodes : Vector.t char 3 :=
+  [WO~0~0~0~0~0~0~0~1;
+   WO~0~0~0~0~0~1~1~0;
+   WO~0~0~0~1~0~0~0~1
   ].
 
-Variable IPChecksum : ByteString -> ByteString.
+Variable onesComplement : list char -> word 16.
+
+Fixpoint transformer_pop_word {B}
+         {transformer : Transformer B}
+         {transformer_opt : TransformerUnitOpt transformer bool}
+         (sz : nat)
+         (b : B)
+  : (word sz * B) :=
+  match sz with
+  | 0 => (WO, b)
+  | S sz' =>
+    match transform_pop_opt b with
+    | Some (v, b') =>
+      let (w', b'') := transformer_pop_word sz' b' in
+      (WS v w', b'')
+    | _ => (wzero (S sz'), b)
+    end
+  end.
+
+Fixpoint ByteString2ListOfChar (n : nat)
+           (b : ByteString) : list char :=
+  match n with
+  | 0 => nil
+  | S n' =>
+    let (c, b') := transformer_pop_word 8 b in
+    cons c (ByteString2ListOfChar n' b')
+  end.
+
+Definition IPChecksum (b : ByteString) : ByteString :=
+  encode_word' _ (onesComplement
+                    match padding b with
+                    | 0 => ByteString2ListOfChar (length (byteString b)) b
+                    | _ => ByteString2ListOfChar (1 + length (byteString b)) b
+                    end).
 
 Definition transformer : Transformer ByteString := ByteStringTransformer.
 
@@ -80,37 +113,243 @@ Definition encode_IPv4_Packet_Spec (ip4 : IPv4_Packet)  :=
 Definition IPv4_Packet_OK (ipv4 : IPv4_Packet) :=
   lt (|ipv4!"Options"|) 11 /\ lt (20 + 4 * |ipv4!"Options"|) (wordToNat ipv4!"TotalLength").
 
-Variable IPChecksum_Valid : nat -> ByteString -> Prop.
-Variable IPChecksum_Valid_dec : forall n b, {IPChecksum_Valid n b} + {~IPChecksum_Valid n b}.
-Variable decodeChecksum : ByteString -> CacheDecode -> option (() * ByteString * CacheDecode).
+Definition IPChecksum_Valid (n : nat) (b : ByteString) : Prop :=
+  onesComplement (ByteString2ListOfChar n b) = wones 16.
 
-Variable IPChecksum_OK : forall b ext : ByteString, IPChecksum_Valid (bin_measure (transform b (IPChecksum b))) (transform (transform b (IPChecksum b)) ext).
+Definition IPChecksum_Valid_dec (n : nat) (b : ByteString)
+  : {IPChecksum_Valid n b} + {~IPChecksum_Valid n b} := weq _ _.
 
-Variable IPChecksum_commute : forall b b' : ByteString, IPChecksum (transform b b') = IPChecksum (transform b' b).
+Definition decode_IPChecksum
+  : ByteString -> CacheDecode -> option (() * ByteString * CacheDecode) :=
+  decode_unused_word 16.
 
-Variable IPChecksum_Valid_commute :
-  forall b b' ext : ByteString,
-    IPChecksum_Valid (bin_measure (transform b b')) (transform (transform b b') ext) <-> IPChecksum_Valid (bin_measure (transform b' b)) (transform (transform b' b) ext).
-
-Variable IPv4_Packet_encoded_measure  : ByteString -> nat.
-
-Lemma IPv4_Packet_encoded_measure_OK :
-  forall (a : IPv4_Packet) (ctx ctx' : ()) (b ext : ByteString),
-    encode_IPv4_Packet_Spec a ctx ↝ (b, ctx')
-    -> length_ByteString b = IPv4_Packet_encoded_measure (ByteString_transformer b ext).
+Lemma IPChecksum_OK :
+  forall (b ext : ByteString),
+    IPChecksum_Valid (bin_measure (transform b (IPChecksum b)))
+                     (transform (transform b (IPChecksum b)) ext).
+Proof.
+  simpl; intros.
 Admitted.
 
-Lemma decodeIPChecksum_pf
+Lemma IPChecksum_commute :
+  forall (b b' : ByteString),
+    IPChecksum (transform b b') = IPChecksum (transform b' b).
+Proof.
+  simpl; intros.
+Admitted.
+
+Lemma IPChecksum_Valid_commute :
+  forall (b b' ext : ByteString),
+    IPChecksum_Valid (bin_measure (transform b b')) (transform (transform b b') ext)
+    <-> IPChecksum_Valid (bin_measure (transform b' b)) (transform (transform b' b) ext).
+Admitted.
+
+Definition IPv4_Packet_encoded_measure (ipv4_b : ByteString)
+  : nat :=
+  match (`(u, b') <- decode_unused_word' 4 ipv4_b;
+           decode_word' 4 b') with
+  | Some n => 32 * wordToNat (fst n)
+  | None => 0
+  end.
+
+Lemma decode_IPChecksum_pf
   : forall (b b' ext : ByteString) (ctx ctx' ctxD : ()),
     True ->
-    decodeChecksum (ByteString_transformer (ByteString_transformer (IPChecksum (ByteString_transformer b b')) b') ext) ctxD = Some ((), ByteString_transformer b' ext, ctxD).
+    decode_IPChecksum (ByteString_transformer (ByteString_transformer (IPChecksum (ByteString_transformer b b')) b') ext) ctxD = Some ((), ByteString_transformer b' ext, ctxD).
+Proof.
+  intros; pose proof transform_assoc as H'; simpl in H'; rewrite <- H'; clear H'.
+  unfold IPChecksum, decode_IPChecksum, decode_unused_word, decode_unused_word'.
+  pose proof transformer_pop_encode_word' as H'; simpl in H'; rewrite H'; simpl; eauto.
+Qed.
+
+Lemma ByteString_pop_eq_push
+  : forall b b' b'',
+    ByteString_pop b = Some (b', b'')
+    -> b = ByteString_push b' b''.
+Proof.
+  destruct b; unfold ByteString_pop; simpl.
+  destruct padding; simpl.
+  - destruct byteString; simpl; intros.
+    + discriminate.
+    + injections.
+      unfold ByteString_push; simpl.
+      f_equal.
+      rewrite (shatter_word front); reflexivity.
+      eapply le_uniqueness_proof.
+      rewrite (shatter_word c); simpl; f_equal.
+  - intros; rewrite (shatter_word front); injections.
+    unfold ByteString_push; simpl.
+    destruct (Peano_dec.eq_nat_dec padding 7).
+    subst; elimtype False; omega.
+    f_equal.
+    eapply le_uniqueness_proof.
+Qed.
+
+Lemma decode_IPChecksum_pf'
+  : forall (u : ()) (b b' : ByteString),
+    () -> forall ctxD ctxD' : (), True -> decode_IPChecksum b ctxD = Some (u, b', ctxD') -> True /\ (exists b'' : ByteString, b = ByteString_transformer b'' b').
+Proof.
+  unfold IPChecksum, decode_IPChecksum, decode_unused_word, decode_unused_word'.
+  intros; destruct (WordOpt.transformer_pop_word 16 b) eqn : ? ;
+    simpl in H1; try discriminate.
+  injections.
+  intuition eauto.
+  simpl in Heqo.
+  pose proof ByteString_transform_push_step_opt as H''; simpl in H''.
+  repeat match goal with
+    H : context[ByteString_pop ?b] |- _ =>
+    let H' := fresh in
+    let b := fresh in
+    destruct (ByteString_pop b) as [ [b ?] | ] eqn : H';
+      try discriminate;
+      eapply ByteString_pop_eq_push in H';
+      rewrite H'; clear H'
+  end; intros.
+  injections.
+  simpl.
+  eexists (ByteString_push H2
+       (ByteString_push H3
+          (ByteString_push H4
+             (ByteString_push H5
+                (ByteString_push H6
+                   (ByteString_push H7
+                      (ByteString_push H8
+                         (ByteString_push H9
+                            (ByteString_push H10
+                               (ByteString_push H11
+                                  (ByteString_push H12
+                                     (ByteString_push H13
+                                        (ByteString_push H14
+                                           (ByteString_push H15
+                                              (ByteString_push H16 (ByteString_push H17 transform_id)))))))))))))))).
+  rewrite !H''; reflexivity.
 Admitted.
 
-Lemma decodeIPChecksum_pf'
-  : forall (u : ()) (b b' : ByteString),
-    () -> forall ctxD ctxD' : (), True -> decodeChecksum b ctxD = Some (u, b', ctxD') -> True /\ (exists b'' : ByteString, b = ByteString_transformer b'' b').
+Lemma length_encode_word' sz :
+  forall (w : word sz), bin_measure (encode_word' sz w) = sz.
 Proof.
-Admitted.
+  induction sz; intros;
+    rewrite (shatter_word w); simpl.
+  - pose proof (transform_measure transform_id transform_id) as H';
+      rewrite transform_id_left in H'.
+    simpl bin_measure in H'; simpl transform_id in H'; omega.
+  - pose proof measure_push as H'; simpl in H'.
+    rewrite H', IHsz; omega.
+Qed.
+
+Lemma IPv4_Packet_encoded_measure_OK :
+  forall (a : IPv4_Packet) (ctx ctx' : ()) (b ext : ByteString)
+         (a_OK : IPv4_Packet_OK a),
+    encode_IPv4_Packet_Spec a ctx ↝ (b, ctx')
+    -> length_ByteString b = IPv4_Packet_encoded_measure (ByteString_transformer b ext).
+Proof.
+  unfold encode_IPv4_Packet_Spec, composeChecksum, compose, Bind2; intros.
+  revert H; pose_string_ids; simpl; intros.
+  repeat apply refine_bind_bind' in H.
+  apply Bind_inv in H; destruct_ex; split_and.
+  repeat apply refine_bind_bind' in H1.
+  apply Bind_inv in H1; destruct_ex; split_and.
+  repeat apply refine_bind_bind' in H2.
+  apply Bind_inv in H2; destruct_ex; split_and.
+  apply refine_bind_unit' in H3.
+  repeat apply refine_bind_bind' in H3.
+  apply Bind_inv in H3; destruct_ex; split_and.
+  repeat apply refine_bind_bind' in H4.
+  apply Bind_inv in H4; destruct_ex; split_and.
+  repeat apply refine_bind_bind' in H5.
+  apply Bind_inv in H5; destruct_ex; split_and.
+  apply refine_bind_unit' in H6.
+  repeat apply refine_bind_bind' in H6.
+  apply Bind_inv in H6; destruct_ex; split_and.
+  repeat apply refine_bind_bind' in H7.
+  apply Bind_inv in H7; destruct_ex; split_and.
+  repeat apply refine_bind_bind' in H8.
+  apply Bind_inv in H8; destruct_ex; split_and.
+  repeat apply refine_bind_bind' in H9.
+  apply Bind_inv in H9; destruct_ex; split_and.
+  repeat apply refine_bind_bind' in H10.
+  apply Bind_inv in H10; destruct_ex; split_and.
+  repeat apply refine_bind_bind' in H11.
+  repeat apply refine_bind_unit' in H11.
+  simpl in H11.
+  repeat apply refine_bind_bind' in H11.
+  apply Bind_inv in H11; destruct_ex; split_and.
+  computes_to_inv.
+  simpl in *.
+  injections.
+  simpl.
+  rewrite !transform_ByteString_measure.
+  unfold IPChecksum.
+  rewrite !length_encode_word'.
+  unfold IPv4_Packet_encoded_measure.
+  unfold encode_word_Spec in H0.
+  computes_to_inv.
+  rewrite <- H0.
+  simpl fst.
+  pose proof transform_assoc as H'; simpl in H'.
+  rewrite <- !H'.
+  simpl fst.
+  unfold decode_unused_word'.
+  pose proof transformer_pop_encode_word' as H''; simpl in H''.
+  unfold fst.
+  rewrite H''.
+  unfold DecodeBindOpt.
+  unfold If_Opt_Then_Else.
+  unfold snd.
+  unfold encode_nat_Spec, encode_word_Spec in H1.
+  computes_to_inv; rewrite <- H1.
+  rewrite <- transformer_pop_word_eq_decode_word'.
+  rewrite H''.
+  unfold encode_word_Spec in *.
+  computes_to_inv.
+  subst.
+  rewrite !length_encode_word'.
+  unfold encode_bool_Spec in *.
+  computes_to_inv.
+  subst.
+  let H' := fresh in
+  pose proof measure_push as H'; simpl in H'; rewrite !H'.
+  simpl transform_id; unfold ByteString_id; simpl length_ByteString.
+  unfold length_ByteString at 1; simpl padding; simpl byteString.
+  unfold length_ByteString at 1; simpl padding; simpl byteString.
+  simpl length.
+  unfold encode_enum_Spec, encode_word_Spec in H10;
+    computes_to_inv.
+  subst.
+  rewrite !length_encode_word'.
+  unfold length_ByteString at 1; simpl padding; simpl byteString.
+  unfold length_ByteString at 2; simpl padding; simpl byteString.
+  simpl length.
+  destruct v3.
+  let H' := fresh in
+  pose proof (measure_encode_length_Spec (A := word 32)) as H';
+    eapply H' in H12'1.
+  2: clear; intros; computes_to_inv; injections;
+    apply length_encode_word'.
+  simpl bin_measure in H12'1.
+  rewrite H12'1.
+  rewrite wordToNat_natToWord_idempotent.
+  rewrite !Mult.mult_0_r.
+  rewrite <- !plus_n_O.
+  rewrite !plus_O_n.
+  omega.
+  unfold IPv4_Packet_OK in a_OK.
+  destruct a_OK.
+  revert H1; clear.
+  simpl.
+  rewrite <- BinNat.N.compare_lt_iff.
+  rewrite Nnat.N2Nat.inj_compare.
+  rewrite <- Znat.positive_nat_N.
+  rewrite !Pnat.Pos2Nat.inj_succ.
+  rewrite Nnat.Nat2N.id.
+  rewrite Pnat.SuccNat2Pos.id_succ.
+  rewrite <- Compare_dec.nat_compare_lt.
+  simpl.
+  unfold BinPos.Pos.to_nat; simpl.
+  unfold StringId11.
+  simpl.
+  auto with arith.
+Admitted. (* Qed takes forever on this proof. *)
 
 Transparent pow2.
 Arguments pow2 : simpl never.
@@ -129,13 +368,13 @@ Proof.
   unfold encode_IPv4_Packet_Spec; pose_string_ids.
   let p := (eval unfold Domain in (fun ip4 : IPv4_Packet => (|ip4!StringId11|, (ip4!StringId, (ip4!StringId0, (ip4!StringId1,
                                                                                                                (ip4!StringId2, (ip4!StringId3, (ip4!StringId4, ip4!StringId5))))))))) in
-  let p := eval simpl in p in 
+  let p := eval simpl in p in
       eapply (@composeChecksum_encode_correct
                 IPv4_Packet _ transformer IPChecksum
                 IPChecksum_Valid IPChecksum_Valid_dec
                 IPChecksum_OK IPChecksum_commute IPChecksum_Valid_commute _
                 (nat * (word 16 * (word 16 * (bool * (bool * (word 13 * (char * EnumType ["ICMP"; "TCP"; "UDP"])))))))
-                _ _ _ decodeChecksum H
+                _ _ _ decode_IPChecksum H
                 p
                 (IPv4_Packet_OK)
                 _ _ _
@@ -153,7 +392,8 @@ Proof.
                                    ThenC encode_enum_Spec ProtocolTypeCodes (snd (snd (snd (snd (snd (snd (snd data')))))))
                                    DoneC))).
   simpl.
-  intros; eapply IPv4_Packet_encoded_measure_OK; apply H0.
+  idtac.
+  intros; eapply IPv4_Packet_encoded_measure_OK; eassumption.
   apply_compose.
   eapply Word_decode_correct.
   solve_data_inv.
@@ -247,8 +487,8 @@ Proof.
   revert H; unfold StringId11; unfold pow2; simpl; auto with arith.
   instantiate (1 := fun _ _ => True);
     simpl; intros; exact I.
-  intros; eapply decodeIPChecksum_pf; eauto.
-  intros; eapply decodeIPChecksum_pf'; eauto.
+  intros; eapply decode_IPChecksum_pf; eauto.
+  intros; eapply decode_IPChecksum_pf'; eauto.
   apply_compose.
   eapply Word_decode_correct.
   solve_data_inv.
